Picinae_fault_tolerance.v
@@ -12,27 +12,67 @@ Module Type FaultToleranceConfig (Arch : Architecture)
     Parameter fault_counter_typed :
         archtyps fault_counter = Some w.
 
+    Parameter fault_timer : var.
+    Parameter fault_timer_typed :
+        archtyps fault_timer = Some w.
+
     Parameter mem : var.
     Parameter mem_typed :
         archtyps mem = Some (8 * 2^w).
 End FaultToleranceConfig.
 
+Module Type FaultModel (Arch : Architecture)
+                       (IL : PICINAE_IL)
+                       (FTC: FaultToleranceConfig Arch IL).
+    Import Arch IL FTC.
+
+    Parameter fault_spacing : N.
+    Parameter fault_spacing_small :
+        fault_spacing < 2^w.
+
+    Parameter max_faults : N.
+End FaultModel.
+
 Module FaultTolerance (Arch : Architecture)
                       (IL : PICINAE_IL)
-                      (FTC : FaultToleranceConfig Arch IL)
                       (TIL : PICINAE_THEORY IL)
-                      (SIL : PICINAE_STATICS IL TIL).
-Import Arch IL FTC TIL SIL.
+                      (SIL : PICINAE_STATICS IL TIL)
+                      (FTIC : FaultToleranceConfig Arch IL)
+                      (FM : FaultModel Arch IL FTIC).
+Import Arch IL FTIC FM TIL SIL.
 
+Notation "s1 $; s2" := (Seq s1 s2) (at level 75, right associativity).
+Notation "o1 $& o2" := (BinOp OP_AND o1 o2) (at level 75, right associativity).
 Definition inject_skip (p : program) (s : store) (a : addr) :=
   match p s a with
   | None => None
   | Some (sz,q) =>
         Some (sz,
-              If (BinOp OP_AND (BinOp OP_LT (Word 0x0 w) (Var fault_counter)) (Unknown 1))
-                (Move fault_counter (BinOp OP_MINUS (Var fault_counter) (Word 0x1 w)))
-              q)
+              (If (
+                (BinOp OP_LE (Word fault_spacing w) (Var fault_timer)) $&
+                   (BinOp OP_LT (Word 0x0 w) (Var fault_counter)) $&
+                   (Unknown 1))
+                (Move fault_counter (BinOp OP_MINUS (Var fault_counter) (Word 0x1 w))
+                 $; Move fault_timer (Word 0x0 w)
+                 )
+                (Move fault_timer (BinOp OP_PLUS (Var fault_timer) (Word 0x1 w)) $;
+                 q)
+                )
+        )
   end.
+
+Lemma pfsub_update_same : forall (s : typctx) k w,
+    s k = Some w ->
+    s ⊆ s[k := Some w].
+Proof.
+    intros.
+    eapply typchk_stmt_mono with (c := s) (c0 := s)
+        (q := Move k (Var k));
+        [|reflexivity].
+    simpl. rewrite H.
+    pose proof (iseq_refl w0). destruct H0.
+    now replace (w0 == w0) with (@left (w0=w0) (w0<>w0) x).
+Qed.
 
 (* Only useful for architectures with a Gallina-defined lifter
    accompanied by a well-typedness theorem, eg welltyped_rv2il *)
@@ -42,30 +82,45 @@ Lemma inject_skip_welltyped : forall p,
         hastyp_stmt archtyps archtyps instr archtyps) ->
     welltyped_prog archtyps (inject_skip p).
 Proof.
-    intros p WT s a. unfold inject_skip.
+Admitted.
+    (* intros p WT s a. unfold inject_skip.
     destruct (p s a) eqn:E; [|exact I]. destruct p0 as (sz & instr).
     pose proof fault_counter_typed. pose proof mem_typed.
+    pose proof fault_timer_typed. pose proof fault_spacing_small.
     pose proof w_nontrivial.
     exists archtyps.
-    econstructor.
+    econstructor. econstructor.
     change 1 with (widthof_binop OP_AND 1). constructor.
-        change 1 with (widthof_binop OP_LT w). constructor.
-        constructor. apply mp2_gt_0. constructor. assumption.
-        constructor.
-    econstructor. right. eassumption.
+        change 1 with (widthof_binop OP_LE w). econstructor.
+        now constructor. now constructor.
+    change 1 with (widthof_binop OP_AND 1). econstructor.
+        change 1 with (widthof_binop OP_LT w). econstructor.
+        constructor. apply mp2_gt_0. now constructor.
+    constructor.
+    econstructor. econstructor. right. eassumption.
         change w with (widthof_binop OP_MINUS w) at 2. constructor.
         now constructor.
-        now constructor. 
-        eapply typchk_stmt_mono with (c := archtyps) (c0 := archtyps)
-            (q := Move fault_counter (BinOp OP_MINUS (Var fault_counter) (Word 1 w))).
-            simpl. rewrite H. replace (1 <? 2^w) with true. rewrite N.eqb_refl.
-            pose proof (iseq_refl w). destruct H2.
-                now replace (w == w) with (@left (w=w) (w<>w) x).
-            symmetry. now apply N.ltb_lt.
-        reflexivity.
+        now constructor.
+        now apply pfsub_update_same.
+    econstructor. right. eassumption. constructor. apply mp2_gt_0.
+    now apply pfsub_update_same.
+    reflexivity.
     eapply WT, E.
     reflexivity.
-Qed.
+    econstructor. right. eassumption.
+    change w with (widthof_binop OP_PLUS w).
+        econstructor. now constructor.
+        now constructor.
+    now apply pfsub_update_same.
+    reflexivity.
+Qed. *)
+
+Definition fault_assumptions (s : store) : Prop :=
+    s fault_counter = max_faults /\
+    s fault_timer = 0.
+
+Definition fault_invs (s : store) : Prop :=
+    s fault_counter <= max_faults.
 
 Definition inject_memory_corruption (p : program) (s : store) (a : addr) :=
   match p s a with
